disk-betree/Graph.dfy
@@ -12,6 +12,7 @@ module ReferenceType {
 
   export S provides Reference, Root, toRef, toUint64, NativeTypes
   export extends S
+	export Internal reveals *
 }
   
 abstract module Graph {
